Massive rework of the provider to support static configurations

providers/evercrypt/c/evercrypt_openssl.c
@@ -1,6 +1,4 @@
-#ifndef NO_OPENSSL
 #include <openssl/evp.h>
-#endif
 #include <inttypes.h>
 
 #include "kremlin/internal/target.h"
@@ -18,22 +16,6 @@
   do {                                                                         \
     KRML_HOST_EPRINTF("Error at %s:%d\n", __FILE__, __LINE__);                   \
   } while (0)
-
-#ifdef NO_OPENSSL
-
-void EverCrypt_OpenSSL_aes256_gcm_encrypt(uint8_t *ciphertext,
-                                          uint8_t *tag,
-                                          uint8_t *key,
-                                          uint8_t *iv,
-                                          uint8_t *plaintext,
-                                          uint32_t plaintext_len,
-                                          uint8_t *aad,
-                                          uint32_t aad_len) {
-  KRML_HOST_EPRINTF("OpenSSL not available in this build\n");
-  KRML_HOST_EXIT(255);
-}
-
-#else
 
 void EverCrypt_OpenSSL_aes256_gcm_encrypt(uint8_t *ciphertext,
                                           uint8_t *tag,
@@ -95,5 +77,3 @@ void EverCrypt_OpenSSL_aes256_gcm_encrypt(uint8_t *ciphertext,
 
   return;
 }
-
-#endif
