providers/evercrypt/c/evercrypt_vale_glue.c
@@ -2,7 +2,7 @@
 #include <stdlib.h>
 
 #include "kremlin/internal/target.h"
-#include "EverCrypt_Vale.h"
+#include "EverCrypt_ValeGlue.h"
 
 // This is SUPER stale and the .h can't even be generated anymore for the module
 // called Vale.Hash.SHA2_256.fst -- currently in secure_api/vale. Rather than
@@ -14,26 +14,26 @@ void Vale_Hash_SHA2_256_update_last(uint32_t *state, uint8_t *data, uint32_t len
 void Vale_Hash_SHA2_256_finish(uint32_t *state, uint8_t *dst);
 void Vale_Hash_SHA2_256_hash(uint32_t *dst, uint8_t *data, uint32_t len);
 
-void EverCrypt_Vale_sha256_init(uint32_t *x0){
+void EverCrypt_ValeGlue_sha256_init(uint32_t *x0){
   Vale_Hash_SHA2_256_init(x0);
 }
 
-void EverCrypt_Vale_sha256_update(uint32_t *x0, uint8_t *x1){
+void EverCrypt_ValeGlue_sha256_update(uint32_t *x0, uint8_t *x1){
   Vale_Hash_SHA2_256_update(x0, x1);
 }
 
-void EverCrypt_Vale_sha256_update_multi(uint32_t *x0, uint8_t *x1, uint32_t x2){
+void EverCrypt_ValeGlue_sha256_update_multi(uint32_t *x0, uint8_t *x1, uint32_t x2){
   for (uint32_t i = 0; i < x2; i++) {
     uint8_t *b = x1 + i * 64;
     Vale_Hash_SHA2_256_update(x0, b);
   }
 }
 
-void EverCrypt_Vale_sha256_update_last(uint32_t *x0, uint8_t *x1, uint32_t x2){
+void EverCrypt_ValeGlue_sha256_update_last(uint32_t *x0, uint8_t *x1, uint32_t x2){
   Vale_Hash_SHA2_256_update_last(x0, x1, x2);
 }
 
-void EverCrypt_Vale_sha256_finish(uint32_t *x0, uint8_t *x1){
+void EverCrypt_ValeGlue_sha256_finish(uint32_t *x0, uint8_t *x1){
   Vale_Hash_SHA2_256_finish(x0, x1);
   // Reverse byte-order in little-endian hosts
   for (int i = 0; i < 8; i++) {
@@ -42,7 +42,7 @@ void EverCrypt_Vale_sha256_finish(uint32_t *x0, uint8_t *x1){
   }
 }
 
-void EverCrypt_Vale_sha256_hash(uint8_t *x0, uint8_t *x1, uint32_t x2){
+void EverCrypt_ValeGlue_sha256_hash(uint8_t *x0, uint8_t *x1, uint32_t x2){
   KRML_HOST_EPRINTF("TODO: sha256_hash/Vale\n");
   KRML_HOST_EXIT(255);
 }
