providers/evercrypt/EverCrypt.Vale.fsti
@@ -1,0 +1,26 @@
+module EverCrypt.Vale
+
+module N = C.Nullity
+
+open EverCrypt.Helpers
+
+/// This module directly exposes "raw" functions, using attributes to make sure
+/// KreMLin generates the right "extern stdcall" declarations. There is no C code to implement this module, the implementations are provided at link-time.
+
+noeq
+type gcm_args = {
+  plain: uint8_p;
+  plain_len: uint64_t;
+  aad: uint8_p;
+  aad_len: uint64_t;
+  iv: uint8_p;
+  expanded_key: uint8_p;
+  cipher: uint8_p;
+  tag: uint8_p;
+}
+
+[@ (CCConv "stdcall") ]
+val gcm_encrypt: N.pointer gcm_args -> Stack_ unit
+
+[@ (CCConv "stdcall") ]
+val aes_key_expansion: key_ptr:uint8_p -> expanded_key_ptr: uint8_p -> uint8_p -> Stack_ unit
