providers/evercrypt/config/default/EverCrypt.StaticConfig.fst
@@ -1,0 +1,5 @@
+module EverCrypt.StaticConfig
+
+inline_for_extraction let hacl = true
+inline_for_extraction let vale = true
+inline_for_extraction let openssl = true
