providers/evercrypt/config/noopenssl/EverCrypt.StaticConfig.fst
@@ -1,0 +1,8 @@
+module EverCrypt.StaticConfig
+
+/// This module allows us to statically eliminate symbols from the resulting
+/// library by setting, for instance, openssl to false.
+
+inline_for_extraction let hacl = true
+inline_for_extraction let vale = true
+inline_for_extraction let openssl = false
