providers/evercrypt/fst/EverCrypt.fst
@@ -1,0 +1,208 @@
+module EverCrypt
+
+module B = FStar.Buffer
+
+module Hacl = EverCrypt.Hacl
+module Vale = EverCrypt.Vale
+module ValeGlue = EverCrypt.ValeGlue
+
+module SC = EverCrypt.StaticConfig
+module AC = EverCrypt.AutoConfig
+
+open EverCrypt.Helpers
+open C.Failure
+
+/// Some remarks here.
+///
+/// - Eta-expanding helps avoid KreMLin errors down the line (and is more
+///   efficient in C.)
+/// - The if-then-else as opposed to a match allows F* to specialize these when
+///   we do a static configuration.
+/// - This file must be maintained in sync with evercrypt_autoconfig.c
+let sha256_init state =
+  let i = AC.sha256_impl () in
+  if SC.hacl && i = AC.Hacl then
+    Hacl.sha256_init state
+  else if SC.vale && i = AC.Vale then
+    ValeGlue.sha256_init state
+  else
+    failwith !$"ERROR: inconsistent configuration"
+
+let sha256_update state data =
+  let i = AC.sha256_impl () in
+  if SC.hacl && i = AC.Hacl then
+    Hacl.sha256_update state data
+  else if SC.vale && i = AC.Vale then
+    ValeGlue.sha256_update state data
+  else
+    failwith !$"ERROR: inconsistent configuration"
+
+let sha256_update_multi state data n =
+  let i = AC.sha256_impl () in
+  if SC.hacl && i = AC.Hacl then
+    Hacl.sha256_update_multi state data n
+  else if SC.vale && i = AC.Vale then
+    ValeGlue.sha256_update_multi state data n
+  else
+    failwith !$"ERROR: inconsistent configuration"
+
+let sha256_update_last state data n =
+  let i = AC.sha256_impl () in
+  if SC.hacl && i = AC.Hacl then
+    Hacl.sha256_update_last state data n
+  else if SC.vale && i = AC.Vale then
+    ValeGlue.sha256_update_last state data n
+  else
+    failwith !$"ERROR: inconsistent configuration"
+
+let sha256_finish state data =
+  let i = AC.sha256_impl () in
+  if SC.hacl && i = AC.Hacl then
+    Hacl.sha256_finish state data
+  else if SC.vale && i = AC.Vale then
+    ValeGlue.sha256_finish state data
+  else
+    failwith !$"ERROR: inconsistent configuration"
+
+let sha256_hash dst src len =
+  let i = AC.sha256_impl () in
+  if SC.hacl && i = AC.Hacl then
+    Hacl.sha256_hash dst src len
+  else if SC.hacl && i = AC.Vale then
+    ValeGlue.sha256_hash dst src len
+  else
+    failwith !$"ERROR: inconsistent configuration"
+
+let sha384_init state =
+  let i = AC.sha384_impl () in
+  if SC.hacl && i = AC.Hacl then
+    Hacl.sha384_init state
+  else
+    failwith !$"ERROR: inconsistent configuration"
+
+let sha384_update state data =
+  let i = AC.sha384_impl () in
+  if SC.hacl && i = AC.Hacl then
+    Hacl.sha384_update state data
+  else
+    failwith !$"ERROR: inconsistent configuration"
+
+let sha384_update_multi state data n =
+  let i = AC.sha384_impl () in
+  if SC.hacl && i = AC.Hacl then
+    Hacl.sha384_update_multi state data n
+  else
+    failwith !$"ERROR: inconsistent configuration"
+
+let sha384_update_last state data n =
+  let i = AC.sha384_impl () in
+  if SC.hacl && i = AC.Hacl then
+    Hacl.sha384_update_last state data n
+  else
+    failwith !$"ERROR: inconsistent configuration"
+
+let sha384_finish state data =
+  let i = AC.sha384_impl () in
+  if SC.hacl && i = AC.Hacl then
+    Hacl.sha384_finish state data
+  else
+    failwith !$"ERROR: inconsistent configuration"
+
+let sha384_hash dst src len =
+  let i = AC.sha384_impl () in
+  if SC.hacl && i = AC.Hacl then
+    Hacl.sha384_hash dst src len
+  else
+    failwith !$"ERROR: inconsistent configuration"
+
+let sha512_init state =
+  let i = AC.sha512_impl () in
+  if SC.hacl && i = AC.Hacl then
+    Hacl.sha512_init state
+  else
+    failwith !$"ERROR: inconsistent configuration"
+
+let sha512_update state data =
+  let i = AC.sha512_impl () in
+  if SC.hacl && i = AC.Hacl then
+    Hacl.sha512_update state data
+  else
+    failwith !$"ERROR: inconsistent configuration"
+
+let sha512_update_multi state data n =
+  let i = AC.sha512_impl () in
+  if SC.hacl && i = AC.Hacl then
+    Hacl.sha512_update_multi state data n
+  else
+    failwith !$"ERROR: inconsistent configuration"
+
+let sha512_update_last state data n =
+  let i = AC.sha512_impl () in
+  if SC.hacl && i = AC.Hacl then
+    Hacl.sha512_update_last state data n
+  else
+    failwith !$"ERROR: inconsistent configuration"
+
+let sha512_finish state data =
+  let i = AC.sha512_impl () in
+  if SC.hacl && i = AC.Hacl then
+    Hacl.sha512_finish state data
+  else
+    failwith !$"ERROR: inconsistent configuration"
+
+let sha512_hash dst src len =
+  let i = AC.sha512_impl () in
+  if SC.hacl && i = AC.Hacl then
+    Hacl.sha512_hash dst src len
+  else
+    failwith !$"ERROR: inconsistent configuration"
+
+let x25519 dst secret base =
+  let i = AC.x25519_impl () in
+  if SC.hacl && i = AC.Hacl then
+    Hacl.x25519 dst secret base
+  else
+    failwith !$"ERROR: inconsistent configuration"
+
+let aes256_gcm_encrypt cipher tag key iv plaintext len ad adlen =
+  let i = AC.aes256_gcm_impl () in
+  if SC.vale && i = AC.Vale then begin
+    push_frame ();
+    let open EverCrypt.Vale in
+    let b = B.create ({
+      plain = plaintext;
+      plain_len = FStar.Int.Cast.Full.uint32_to_uint64 len;
+      aad = ad;
+      aad_len = FStar.Int.Cast.Full.uint32_to_uint64 adlen;
+      iv = iv;
+      expanded_key = key;
+      cipher = cipher;
+      tag = tag
+    }) 1ul in
+    Vale.gcm_encrypt b;
+    pop_frame ()
+  end else if SC.openssl && i = AC.OpenSSL then
+    EverCrypt.OpenSSL.aes256_gcm_encrypt cipher tag key iv plaintext len ad adlen
+  else
+    failwith !$"ERROR: inconsistent configuration"
+
+let chacha20_poly1305_encode_length lb aad_len m_len =
+  let i = AC.chacha20_poly1305_impl () in
+  if SC.hacl && i = AC.Hacl then
+    EverCrypt.Hacl.chacha20_poly1305_encode_length lb aad_len m_len
+  else
+    failwith !$"ERROR: inconsistent configuration"
+
+let chacha20_poly1305_encrypt c mac m m_len aad aad_len k n =
+  let i = AC.chacha20_poly1305_impl () in
+  if SC.hacl && i = AC.Hacl then
+    EverCrypt.Hacl.chacha20_poly1305_encrypt c mac m m_len aad aad_len k n
+  else
+    failwith !$"ERROR: inconsistent configuration"
+
+let chacha20_poly1305_decrypt m c m_len mac aad aad_len k n  =
+  let i = AC.chacha20_poly1305_impl () in
+  if SC.hacl && i = AC.Hacl then
+    EverCrypt.Hacl.chacha20_poly1305_decrypt m c m_len mac aad aad_len k n
+  else
+    failwith !$"ERROR: inconsistent configuration"
